Convert bitvector enumerate to vector

Roolean/QfBv/Domain/Bitvector.lean
@@ -81,9 +81,9 @@ public theorem BitvectorDomain.ofBitvector_id {w} (b: Bitvector w) : BitvectorDo
 public theorem BitvectorDomain.toBitvector?_someSelf {w} (b: Bitvector w) : BitvectorDomain.toBitvector? b = some b
   := by simp[BitvectorDomain, Bitvector.toBitvector?]
 
-public def Bitvector.enumerate (w: Nat) : Array (Bitvector w) :=
-  Array.ofFn λ (n: Fin (2^w)) => { value := BitVec.ofFin n }
+public def Bitvector.enumerate (w: Nat) : Vector (Bitvector w) (2^w) :=
+  Vector.ofFn λ (n: Fin (2^w)) => { value := BitVec.ofFin n }
 
 public theorem Bitvector.enumerate_containsAll (w: Nat) (c: Bitvector w)
   : c ∈ Bitvector.enumerate w := by
-  rw[Bitvector.enumerate]; rw[Array.mem_ofFn]; exists c.value.toFin
+  rw[Bitvector.enumerate]; rw[Vector.mem_ofFn]; exists c.value.toFin
